nola/examples/deriv.v
@@ -1,0 +1,318 @@
+(** * Logic with derivability *)
+
+From nola.iris Require Export cif inv_deriv pborrow_deriv.
+From nola.bi Require Import util.
+From nola.heap_lang Require Export notation proofmode lib.mutex.
+From nola.examples Require Export nsynty.
+Import ProdNotation UpdwNotation WpwNotation iPropAppNotation PsemNotation
+  SemNotation ProphNotation LftNotation NsyntyNotation.
+
+Implicit Type (N : namespace) (dq : dfrac) (l : loc) (b : bool) (α β : lft)
+  (q : Qp) (X Y : nsynty).
+
+(** ** Preliminaries *)
+
+(** [sel]: Selector *)
+Variant sel :=
+| (** Points-to token *) cifs_pointsto (l : loc) (dq : dfrac) (v : val)
+| (** Invariant *) cifs_inv (N : namespace)
+| (** Mutex *) cifs_mutex (l : loc)
+| (** Non-prophetic closed borrower *) cifs_borc (α : lft)
+| (** Non-prophetic borrower *) cifs_bor (α : lft)
+| (** Non-prophetic open borrower *) cifs_obor (α : lft) (q : Qp)
+| (** Non-prophetic lender *) cifs_lend (α : lft)
+| (** Prophetic closed borrower *)
+    cifs_pborc {X} (α : lft) (x : X) (ξ : prvar X)
+| (** Prophetic borrower *) cifs_pbor {X} (α : lft) (x : X) (ξ : prvar X)
+| (** Prophetic open borrower *) cifs_pobor {X} (α : lft) (q : Qp) (ξ : prvar X)
+| (** Prophetic lender *) cifs_plend {X} (α : lft) (xπ : clair nsynty X).
+(** [idom]: Domain for inductive parts *)
+Definition idom (_ : sel) : Type := Empty_set.
+(** [cdom]: Domain for coinductive parts *)
+Definition cdom (s : sel) : Type := match s with
+  | cifs_pointsto _ _ _ => Empty_set
+  | cifs_inv _ | cifs_mutex _
+    | cifs_borc _ | cifs_bor _ | cifs_obor _ _ | cifs_lend _ => unit
+  | @cifs_pborc X _ _ _ | @cifs_pbor X _ _ _ | @cifs_pobor X _ _ _
+    | @cifs_plend X _ _ => X
+  end.
+(** [dataOF]: Data [oFunctor] *)
+Definition dataOF (_ : sel) : oFunctor := unitO.
+(** [dataOF] is contractive *)
+Fact dataOF_contractive {s} : oFunctorContractive (dataOF s).
+Proof. exact _. Qed.
+
+(** ** [cif]: Formulas *)
+Notation cif Σ := (cif idom cdom dataOF Σ).
+Notation cifOF := (cifOF idom cdom dataOF).
+
+(** [cifOF] is contractive *)
+Fact cifOF_contractive : oFunctorContractive cifOF.
+Proof. exact _. Qed.
+
+(** Construct [cif] *)
+Section cif.
+  Context {Σ : gFunctors}.
+  Implicit Type Px : cif Σ.
+  (** Points-to token *)
+  Definition cif_pointsto l dq v : cif Σ :=
+    cif_custom (D:=dataOF) (cifs_pointsto l dq v) nullary nullary ().
+  (** Invariant *)
+  Definition cif_inv N Px : cif Σ :=
+    cif_custom (cifs_inv N) nullary (unary Px) ().
+  (** Mutex *)
+  Definition cif_mutex l Px : cif Σ :=
+    cif_custom (cifs_mutex l) nullary (unary Px) ().
+  (** Non-prophetic closed borrower *)
+  Definition cif_borc α Px : cif Σ :=
+    cif_custom (cifs_borc α) nullary (unary Px) ().
+  (** Non-prophetic borrower *)
+  Definition cif_bor α Px : cif Σ :=
+    cif_custom (cifs_bor α) nullary (unary Px) ().
+  (** Non-prophetic open borrower *)
+  Definition cif_obor α q Px : cif Σ :=
+    cif_custom (cifs_obor α q) nullary (unary Px) ().
+  (** Non-prophetic lender *)
+  Definition cif_lend α Px : cif Σ :=
+    cif_custom (cifs_lend α) nullary (unary Px) ().
+  (** Prophetic closed borrower *)
+  Definition cif_pborc {X} α x ξ (Φx : X -d> cif Σ) : cif Σ :=
+    cif_custom (@cifs_pborc X α x ξ) nullary Φx ().
+  (** Prophetic borrower *)
+  Definition cif_pbor {X} α x ξ (Φx : X -d> cif Σ) : cif Σ :=
+    cif_custom (@cifs_pbor X α x ξ) nullary Φx ().
+  (** Prophetic open borrower *)
+  Definition cif_pobor {X} α q ξ (Φx : X -d> cif Σ) : cif Σ :=
+    cif_custom (@cifs_pobor X α q ξ) nullary Φx ().
+  (** Prophetic lender *)
+  Definition cif_plend {X} α xπ (Φx : X -d> cif Σ) : cif Σ :=
+    cif_custom (@cifs_plend X α xπ) nullary Φx ().
+
+  (** The custom constructors are non-expansive *)
+  #[export] Instance cif_inv_ne {N} : NonExpansive (cif_inv N).
+  Proof. move=> ????. apply cif_custom_ne; solve_proper. Qed.
+  #[export] Instance cif_mutex_ne {l} : NonExpansive (cif_mutex l).
+  Proof. move=> ????. apply cif_custom_ne; solve_proper. Qed.
+  #[export] Instance cif_borc_ne {α} : NonExpansive (cif_borc α).
+  Proof. move=> ????. apply cif_custom_ne; solve_proper. Qed.
+  #[export] Instance cif_bor_ne {α} : NonExpansive (cif_bor α).
+  Proof. move=> ????. apply cif_custom_ne; solve_proper. Qed.
+  #[export] Instance cif_obor_ne {α q} : NonExpansive (cif_obor α q).
+  Proof. move=> ????. apply cif_custom_ne; solve_proper. Qed.
+  #[export] Instance cif_lend_ne {α} : NonExpansive (cif_lend α).
+  Proof. move=> ????. apply cif_custom_ne; solve_proper. Qed.
+  #[export] Instance cif_pborc_ne {X α x ξ} : NonExpansive (@cif_pborc X α x ξ).
+  Proof. move=> ????. apply cif_custom_ne; solve_proper. Qed.
+  #[export] Instance cif_pbor_ne {X α x ξ} : NonExpansive (@cif_pbor X α x ξ).
+  Proof. move=> ????. apply cif_custom_ne; solve_proper. Qed.
+  #[export] Instance cif_pobor_ne {X α q ξ} : NonExpansive (@cif_pobor X α q ξ).
+  Proof. move=> ????. apply cif_custom_ne; solve_proper. Qed.
+  #[export] Instance cif_plend_ne {X α xπ} : NonExpansive (@cif_plend X α xπ).
+  Proof. move=> ????. apply cif_custom_ne; solve_proper. Qed.
+End cif.
+Notation "l ↦ dq v" := (cif_pointsto l dq v)
+  (at level 20, dq custom dfrac at level 1, format "l  ↦ dq  v") : cif_scope.
+
+
+(** ** [judg]: Judgment *)
+Definition judg Σ : ofe :=
+  (leibnizO namespace * cif Σ + cif Σ * cif Σ + cif Σ * cif Σ +
+    sigT (A:=nsynty *' nsynty) (λ '(X, Y)',
+      leibnizO (clair nsynty X *' clair nsynty Y) *
+      (X -d> cif Σ) * (Y -d> cif Σ)))%type.
+Definition inv_jacsr {Σ} N Px : judg Σ := inl (inl (inl (N, Px))).
+Definition mutex_jiff {Σ} Px Qx : judg Σ := inl (inl (inr (Px, Qx))).
+Definition pborrow_jto {Σ} Px Qx : judg Σ := inl (inr (Px, Qx)).
+Definition pborrow_jlto {Σ X Y} xπ yπ Φx Ψx : judg Σ :=
+  inr (existT (X, Y)' ((xπ, yπ)', Φx, Ψx)).
+#[export] Instance inv_jacsr_ne {Σ N} : NonExpansive (@inv_jacsr Σ N).
+Proof. move=> ????. by do 3 apply: inl_ne. Qed.
+#[export] Instance mutex_jiff_ne {Σ} : NonExpansive2 (@mutex_jiff Σ).
+Proof. move=> ???????. do 2 apply: inl_ne. exact: inr_ne. Qed.
+#[export] Instance pborrow_jto_ne {Σ} : NonExpansive2 (@pborrow_jto Σ).
+Proof. move=> ???????. apply: inl_ne. exact: inr_ne. Qed.
+#[export] Instance pborrow_jlto_ne {Σ X Y xπ yπ} :
+  NonExpansive2 (@pborrow_jlto Σ X Y xπ yπ).
+Proof.
+  move=> ???????. apply inr_ne. apply: existT_ne=>/=. by split; [split|].
+Qed.
+
+#[export] Instance judg_inv_pre_deriv {Σ} :
+  InvPreDeriv (cif Σ) (judg Σ) := INV_PRE_DERIV inv_jacsr.
+#[export] Instance judg_mutex_pre_deriv {Σ} :
+  MutexPreDeriv (cif Σ) (judg Σ) := MUTEX_PRE_DERIV mutex_jiff.
+#[export] Instance judg_pborrow_pre_deriv {Σ} :
+  PborrowPreDeriv nsynty (cif Σ) (judg Σ) :=
+  PBORROW_PRE_DERIV pborrow_jto (@pborrow_jlto _).
+
+Section sem.
+  Context `{!inv'GS cifOF Σ, !mutexGS cifOF Σ, !pborrowGS nsynty cifOF Σ,
+    !heapGS_gen hlc Σ}.
+  Implicit Type δ : judg Σ → iProp Σ.
+
+  (** ** [bsem]: Base semantics *)
+  Definition bsem δ s :
+    (idom s -d> iProp Σ) → (cdom s -d> cif Σ) → dataOF s $oi Σ → iProp Σ :=
+    match s with
+    | cifs_pointsto l dq v => λ _ _ _, l ↦{dq} v
+    | cifs_inv N => λ _ Pxs _, inv' δ N (Pxs ())
+    | cifs_mutex l => λ _ Pxs _, mutex δ l (Pxs ())
+    | cifs_borc α => λ _ Pxs _, nborc δ α (Pxs ())
+    | cifs_bor α => λ _ Pxs _, nbor δ α (Pxs ())
+    | cifs_obor α q => λ _ Pxs _, nobor δ α q (Pxs ())
+    | cifs_lend α => λ _ Pxs _, nlend δ α (Pxs ())
+    | cifs_pborc α x ξ => λ _ Φx _, pborc δ α x ξ Φx
+    | cifs_pbor α x ξ => λ _ Φx _, pbor δ α x ξ Φx
+    | cifs_pobor α q ξ => λ _ Φx _, pobor δ α q ξ Φx
+    | cifs_plend α xπ => λ _ Φx _, plend δ α xπ Φx
+    end%I.
+
+  (** [bsem] is non-expansive *)
+  #[export] Instance bsem_ne `{!NonExpansive δ} {s} : NonExpansive3 (bsem δ s).
+  Proof. case s; solve_proper. Qed.
+
+  (** Parameterized semantics of [cif] *)
+  #[export] Instance cif_dsem : Dsem (judg Σ) (cif Σ) (iProp Σ) :=
+    DSEM (λ δ, cif_sem (bsem δ)).
+
+  (** [cif_sem] is non-expansive *)
+  Fact cif_sem_ne `{!NonExpansive δ} : NonExpansive ⟦⟧(δ)@{cif Σ}.
+  Proof. exact _. Qed.
+
+  Context `{!heapGS_gen hlc Σ}.
+
+  (** [judg_sem]: Judgment semantics *)
+  Definition judg_sem δ (J : judg Σ) := match J with
+    | inl (inl (inl (N, Px))) => inv_acsr ⟦⟧(δ) N ⟦ Px ⟧(δ)
+    | inl (inl (inr (Px, Qx))) => mod_iff (fupd ⊤ ⊤) ⟦ Px ⟧(δ) ⟦ Qx ⟧(δ)
+    | inl (inr (Px, Qx)) => ⟦ Px ⟧(δ) ==∗ ⟦ Qx ⟧(δ)
+    | inr (existT (X, Y)' ((xπ, yπ)', Φx, Ψx)) =>
+        plend_body ⟦ ⟧(δ) xπ Φx ==∗ plend_body ⟦ ⟧(δ) yπ Ψx
+    end%I.
+  Local Instance judg_sem_ne `{!NonExpansive δ} : NonExpansive (judg_sem δ).
+  Proof.
+    move=> ? _ _[_ _[_ _[|]|]|].
+    - move=> [??][??][/=/leibniz_equiv_iff<- ?]. solve_proper.
+    - move=> [??][??][/=??]. solve_proper.
+    - move=> [??][??]/=[??]. solve_proper.
+    - move=> [?[[[??]?]?]][?[[[??]?]?]][/=?]. subst=>/=.
+      move=> [/=[/=/leibniz_equiv_iff[<-<-]?]?]. solve_proper.
+  Qed.
+  #[export] Instance judg_dsem : Dsem (judg Σ) (judg Σ) (iProp Σ) :=
+    DSEM judg_sem.
+  Canonical judgJ : judgi (iProp Σ) := Judgi (judg Σ).
+
+  #[export] Instance judg_inv_deriv : InvDeriv cifOF Σ judgJ.
+  Proof. done. Qed.
+  #[export] Instance judg_mutex_deriv : MutexDeriv cifOF Σ judgJ.
+  Proof. done. Qed.
+  #[export] Instance judg_pborrow_deriv : PborrowDeriv nsynty cifOF Σ judgJ.
+  Proof. done. Qed.
+End sem.
+
+Section verify.
+  Context `{!inv'GS cifOF Σ, !mutexGS cifOF Σ,
+    !pborrowGS nsynty cifOF Σ, !heapGS_gen hlc Σ}.
+  Implicit Type (Px Qx : cif Σ) (Φx Ψx : loc → cif Σ).
+
+  (** ** Linked list *)
+
+  (** [ilist]: Formula for a list *)
+  Definition ilist_gen N Φx Ilist' l : cif Σ :=
+    cif_inv N (Φx l) ∗ cif_inv N (Ilist' N Φx l).
+  Definition ilist'_gen N Φx Ilist' l : cif Σ :=
+    ∃ l', (l +ₗ 1) ↦ #l' ∗ ilist_gen N Φx Ilist' l'.
+  CoFixpoint ilist' N Φx : loc → cif Σ := ilist'_gen N Φx ilist'.
+  Definition ilist N Φx : loc → cif Σ := ilist_gen N Φx ilist'.
+
+  (** Convert the predicate of [ilist] using [mod_acsr] *)
+  Local Lemma inv'_acsr_iff `{!Deriv ih δ} {N Φx Ψx l} :
+    □ (∀ l' δ', ⌜Deriv ih δ'⌝ → ⌜ih δ'⌝ →
+      mod_acsr (fupd ∅ ∅) ⟦ Φx l' ⟧(δ') ⟦ Ψx l' ⟧(δ') ∧
+      mod_acsr (fupd ∅ ∅) ⟦ Ψx l' ⟧(δ') ⟦ Φx l' ⟧(δ')) ⊢
+      inv' δ N (Φx l) ∗-∗ inv' δ N (Ψx l).
+  Proof.
+    iIntros "#big". iSplit; iApply inv'_acsr; iIntros "!>" (????);
+      [iApply bi.and_elim_l|iApply bi.and_elim_r]; by iApply "big".
+  Qed.
+  Local Lemma inv'_ilist'_iff `{!Deriv ih δ} {N Φx Ψx l} :
+    □ (∀ l' δ', ⌜Deriv ih δ'⌝ → ⌜ih δ'⌝ →
+      inv' δ' N (Φx l') ∗-∗ inv' δ' N (Ψx l')) -∗
+      inv' δ N (ilist' N Φx l) ∗-∗ inv' δ N (ilist' N Ψx l).
+  Proof.
+    move: l. apply Deriv_ind=> δ' ??. iIntros "#eqv".
+    iSplit; iApply inv'_acsr; iIntros "!>" (??[IH ?]?);
+      rewrite -(wand_iff_mod_acsr (M:=fupd _ _)) !/⟦ ilist' _ _ _ ⟧(_);
+      (iModIntro; iSplit; iIntros "/=[%[$[ihd ?]]]"; (iSplit; [|by iApply IH]));
+      iApply ("eqv" with "[%] [//] ihd"); by apply Deriv_mono=> ?[??].
+  Qed.
+  Lemma ilist_acsr `{!Deriv ih δ} {N Φx Ψx l} :
+    □ (∀ l' δ', ⌜Deriv ih δ'⌝ → ⌜ih δ'⌝ →
+      mod_acsr (fupd ∅ ∅) ⟦ Φx l' ⟧(δ') ⟦ Ψx l' ⟧(δ') ∧
+      mod_acsr (fupd ∅ ∅) ⟦ Ψx l' ⟧(δ') ⟦ Φx l' ⟧(δ')) -∗
+      ⟦ ilist N Φx l ⟧(δ) ∗-∗ ⟦ ilist N Ψx l ⟧(δ).
+  Proof.
+    iIntros "#eqv". rewrite /⟦ ⟧(δ) /=.
+    iSplit; (iIntros "[ihd itl]"; iSplitL "ihd";
+      [by iApply (inv'_acsr_iff (Φx:=Φx))|]);
+      iApply (inv'_ilist'_iff with "[] itl"); iIntros "!>" (????);
+      [iApply bi.wand_iff_sym|]; by iApply inv'_acsr_iff.
+  Qed.
+
+  (** ** Linked list with a mutex *)
+
+  (** [mlist]: Formula for a list with a mutex *)
+  Definition mlist_gen Φx Mlist' l : cif Σ :=
+    cif_mutex l (Mlist' Φx l).
+  Definition mlist'_gen Φx Mlist' l : cif Σ :=
+    Φx (l +ₗ 1) ∗ ∃ l', (l +ₗ 2) ↦ #l' ∗ mlist_gen Φx Mlist' l'.
+  CoFixpoint mlist' Φx : loc → cif Σ := mlist'_gen Φx mlist'.
+  Definition mlist Φx : loc → cif Σ := mlist_gen Φx mlist'.
+
+  (** Convert the predicate of [mlist] using [mod_iff] *)
+  Lemma mlist_iff `{!Deriv ih δ} {Φx Ψx l} :
+    □ (∀ l' δ', ⌜Deriv ih δ'⌝ → ⌜ih δ'⌝ →
+      mod_iff (fupd ⊤ ⊤) ⟦ Φx l' ⟧(δ') ⟦ Ψx l' ⟧(δ')) -∗
+      ⟦ mlist Φx l ⟧(δ) ∗-∗ ⟦ mlist Ψx l ⟧(δ).
+  Proof.
+    rewrite !/⟦ mlist _ _ ⟧(_) /=. move: l. apply Deriv_ind=> ???.
+    iIntros "#eqv". iApply mutex_iff. iIntros "!>" (??[IH ?]?).
+    rewrite !/⟦ mlist' _ _ ⟧(_) /=.
+    have ?: Deriv ih δ'. { by apply Deriv_mono=> ?[??]. }
+    iSplit; (iIntros "[hd[%[$ mtl]]]"; iSplitL "hd"; [by iApply "eqv"|]);
+      iModIntro; iRevert "mtl"; [iApply bi.and_elim_l|iApply bi.and_elim_r];
+      by iApply IH.
+  Qed.
+
+  (** ** On derivability *)
+
+  Local Lemma inv'_sep_comm' `{!Deriv ih δ} {N Px Qx} :
+    inv' δ N (Px ∗ Qx)%n ⊢ inv' δ N (Qx ∗ Px)%n.
+  Proof.
+    iApply inv'_iff. iIntros "!>" (????). rewrite /⟦⟧(_) /= bi.sep_comm.
+    iApply bi.wand_iff_refl.
+  Qed.
+  Lemma inv'_sep_comm `{!Deriv ih δ} {N Px Qx} :
+    inv' δ N (Px ∗ Qx)%n ⊣⊢ inv' δ N (Qx ∗ Px)%n.
+  Proof. apply bi.equiv_entails. split; exact inv'_sep_comm'. Qed.
+
+  Local Lemma inv'_inv'_sep_comm' `{!Deriv ih δ} {N N' Px Qx} :
+    inv' δ N (cif_inv N' (Px ∗ Qx)) ⊢ inv' δ N (cif_inv N' (Qx ∗ Px)).
+  Proof.
+    iApply inv'_iff. iIntros "!>" (????). rewrite /⟦⟧(_) /= inv'_sep_comm.
+    iApply bi.wand_iff_refl.
+  Qed.
+  Lemma inv'_inv'_sep_comm `{!Deriv ih δ} {N N' Px Qx} :
+    inv' δ N (cif_inv N' (Px ∗ Qx)) ⊣⊢ inv' δ N (cif_inv N' (Qx ∗ Px)).
+  Proof. apply bi.equiv_entails. split; exact inv'_inv'_sep_comm'. Qed.
+
+  Local Lemma inv'_bor_lft' `{!Deriv ih δ} {N α β Px} :
+    α ⊑□ β -∗ β ⊑□ α -∗ inv' δ N (cif_bor α Px) -∗ inv' δ N (cif_bor β Px).
+  Proof.
+    iIntros "#? #?". iApply inv'_iff. iIntros "!>" (????). rewrite /⟦⟧(_) /=.
+    iSplit; by iApply nbor_lft.
+  Qed.
+  Lemma inv'_bor_lft `{!Deriv ih δ} {N α β Px} :
+    α ⊑□ β -∗ β ⊑□ α -∗ inv' δ N (cif_bor α Px) ∗-∗ inv' δ N (cif_bor β Px).
+  Proof. iIntros "#? #?". iSplit; by iApply inv'_bor_lft'. Qed.
+End verify.
